coq_session/tll_cren.v
@@ -6,6 +6,58 @@ Set Implicit Arguments.
 Unset Strict Implicit.
 Unset Printing Implicit Defensive.
 
+Fixpoint term_cren (m : term) (ξ : cvar -> cvar) : term :=
+  match m with
+  (* core *)
+  | Var x => Var x
+  | Sort s => Sort s
+  | Pi0 A B s => Pi0 (term_cren A ξ) (term_cren B ξ) s
+  | Pi1 A B s => Pi1 (term_cren A ξ) (term_cren B ξ) s
+  | Lam0 A m s => Lam0 (term_cren A ξ) (term_cren m ξ) s
+  | Lam1 A m s => Lam1 (term_cren A ξ) (term_cren m ξ) s
+  | App m n => App (term_cren m ξ) (term_cren n ξ)
+  | Sig0 A B s => Sig0 (term_cren A ξ) (term_cren B ξ) s
+  | Sig1 A B s => Sig1 (term_cren A ξ) (term_cren B ξ) s
+  | Pair0 m n s => Pair0 (term_cren m ξ) (term_cren n ξ) s
+  | Pair1 m n s => Pair1 (term_cren m ξ) (term_cren n ξ) s
+  | LetIn A m n =>
+      LetIn
+        (term_cren A ξ)
+        (term_cren m ξ)
+        (term_cren n ξ)
+  | Fix A m => Fix (term_cren A ξ) (term_cren m ξ)
+  (* data *)
+  | Unit => Unit
+  | II => II
+  | Bool => Bool
+  | TT => TT
+  | FF => FF
+  | Ifte A m n1 n2 =>
+      Ifte
+        (term_cren A ξ)
+        (term_cren m ξ)
+        (term_cren n1 ξ)
+        (term_cren n2 ξ)
+  (* monadic *)
+  | IO A => IO (term_cren A ξ)
+  | Return m => Return (term_cren m ξ)
+  | Bind m n => Bind (term_cren m ξ) (term_cren n ξ)
+  (* session *)
+  | Proto => Proto
+  | Stop r => Stop r
+  | Act0 r A B => Act0 r (term_cren A ξ) (term_cren B ξ)
+  | Act1 r A B => Act1 r (term_cren A ξ) (term_cren B ξ)
+  | Ch r A => Ch r (term_cren A ξ)
+  | CVar x => CVar (ξ x)
+  | Fork A m => Fork (term_cren A ξ) (term_cren m ξ)
+  | Recv0 m => Recv0 (term_cren m ξ)
+  | Recv1 m => Recv1 (term_cren m ξ)
+  | Send0 m => Send0 (term_cren m ξ)
+  | Send1 m => Send1 (term_cren m ξ)
+  | Close m => Close (term_cren m ξ)
+  | Wait m => Wait (term_cren m ξ)
+  end.
+
 Lemma term_cren_ren m ξ ξ' :
   term_cren m.[ren ξ] ξ' = (term_cren m ξ').[ren ξ].
 Proof with eauto.
