coq_session/proc_step.v
@@ -1,6 +1,6 @@
 From mathcomp Require Import ssreflect ssrbool eqtype ssrnat seq.
 From Coq Require Import ssrfun Classical Utf8.
-Require Export AutosubstSsr ARS dyn_weak.
+Require Export AutosubstSsr ARS tll_ast tll_cren.
 
 Set Implicit Arguments.
 Unset Strict Implicit.
@@ -12,125 +12,39 @@ Inductive proc :=
 | Nu (p : proc).
 
 Notation "⟨ m ⟩" := (Exp m).
-Notation "p ∣ q" := (Par p q) (at level 50).
-Notation "'ν.' p" := (Nu p) (at level 50).
+Notation "p ∣ q" := (Par p q) (at level 20).
+Notation "'ν.' p" := (Nu p) (at level 20).
 
+Fixpoint proc_cren (p : proc) (ξ : cvar -> cvar) : proc :=
+  match p with
+  | ⟨ m ⟩ => ⟨ term_cren m ξ ⟩
+  | p ∣ q => (proc_cren p ξ) ∣ (proc_cren q ξ)
+  | ν.p => ν.(proc_cren p (upren (upren ξ)))
+  end.
 
-Lemma dyn_crename Θ Θ' Γ Γ' Δ Δ' m A ξ :
-  Θ ; Γ ; Δ ⊢ m : A -> dyn_agree_cren ξ Θ Γ Δ Θ' Γ' Δ' ->
-  Θ' ; Γ' ; Δ' ⊢ term_cren m ξ : term_cren A ξ.
-Proof with eauto using dyn_empty, dyn_type.
-  move=>ty. elim: ty Θ' Γ' Δ' ξ=>/={Θ Γ Δ m A}.
-  { intros.
-    econstructor.
-    admit.
-    admit.
-    admit.
-    admit. }
-  { intros.
-    econstructor.
-    admit.
-    admit.
-    apply: H2.
-    econstructor.
-    eauto.
-    admit.
-    eauto. }
-  { intros.
-    econstructor.
-    admit.
-    admit.
-    apply: H2.
-    constructor.
-    eauto.
-    admit.
-    eauto. }
-  { intros.
-    rewrite term_cren_beta.
-    apply: dyn_app0...
-    admit. }
-  { intros.
-    rewrite term_cren_beta.
-    apply: dyn_app1...
-    admit.
-    admit.
-    apply: H2.
-    admit.
-    apply: H4.
-    admit. }
-
-Lemma dyn_strengthen Θ m A :
-  _: Θ ; nil ; nil ⊢ term_cren m (+1) : term_cren A (+1) ->
-  Θ ; nil ; nil ⊢ m : A.
-Proof with eauto using dyn_empty, dyn_type.
-  intros.
-  replace m with (term_cren (term_cren m (+1)) (subn^~ 1)).
-  replace A with (term_cren (term_cren A (+1)) (subn^~ 1)).
-  apply: dyn_crename.
-  apply: H.
-  constructor.
-  replace (subn^~ 1) with (id >>> subn^~ 1) by autosubst.
-  constructor.
-  constructor.
-
-
-  move=>ty. elim: ty Γ' Δ'=>//={Θ Γ Δ m A}...
-  admit.
-  { intros.
-    constructor...
-    admit.
-    admit.
-    apply: H2.
-    econstructor...
-    admit. }
-  admit.
-  admit.
-  admit.
-  admit.
-  admit.
-  admit.
-  admit.
-  admit.
-  admit.
-  admit.
-  admit.
-  admit.
-  admit.
-  { intros.
-    replace (term_cren A.[ren (+size Γ)] (+1))
-      with (term_cren A (+1)).[ren (+size Γ')].
-    apply: dyn_cvar.
-    admit.
-    admit.
-    admit.
-    admit.
-    admit. }
-  { intros.
-    econstructor...
-    constructor... }
-  { intros.
-    econstructor...
-    constructor... }
-  { intros.
-  }
-Admitted.
-
-Lemma dyn_cweaken0 Θ m A :
-  Θ ; nil ; nil ⊢ m : A ->
-  _: Θ ; nil ; nil ⊢ term_cren m (+1) : term_cren A (+1).
-Proof with eauto using dyn_empty, dyn_type.
-  intros.
-  apply: dyn_cweaken...
-  constructor.
-
-  move=>ty. elim: ty Γ' Δ'=>//={Θ Γ Δ m A}...
-  { intros.
-    econstructor...
-
-    
-    constructor... }
-  { intros.
-    econstructor...
-    constructor... }
-  { intros.
-  }
+Inductive proc_congr0 : proc -> proc -> Prop :=
+| proc_congr0_par_sym p q :
+  proc_congr0 (p ∣ q) (q ∣ p)
+| proc_congr0_assoc o p q :
+  proc_congr0 (o ∣ (p ∣ q)) ((o ∣ p) ∣ q)
+| proc_congr0_associ o p q :
+  proc_congr0 ((o ∣ p) ∣ q) (o ∣ (p ∣ q)) 
+| proc_congr0_scope p (q : proc) :
+  proc_congr0 ((ν.p) ∣ q) (ν.(p ∣ proc_cren q (+2)))
+| proc_congr0_scopei p (q : proc) :
+  proc_congr0 (ν.(p ∣ proc_cren q (+2))) ((ν.p) ∣ q) 
+| proc_congr0_par p p' q q' :
+  proc_congr0 p p' ->
+  proc_congr0 q q' ->
+  proc_congr0 (p ∣ q) (p' ∣ q')
+| proc_congr0_pari p p' q q' :
+  proc_congr0 p p' ->
+  proc_congr0 q q' ->
+  proc_congr0 (p' ∣ q') (p ∣ q) 
+| proc_congr0_nu p p' :
+  proc_congr0 p p' ->
+  proc_congr0 (ν.p) (ν.p')
+| proc_congr0_nui p p' :
+  proc_congr0 p p' ->
+  proc_congr0 (ν.p') (ν.p).
+Notation "p ≡ q" := (conv proc_congr0 p q) (at level 50).
